

Problem 1

(a)

$$Au = b$$

$$A\hat{u} = \hat{b}$$

$$A(u + \Delta u) = b + \Delta b$$

$$Au + A\Delta u = b + \Delta b$$

$$b + A\Delta u = b + \Delta b$$

$$A\Delta u = \Delta b$$

$$\Delta u = A^{-1}\Delta b$$

$$\|\Delta u\| = \|A^{-1}\Delta b\| \leq \|A^{-1}\| \cdot \|\Delta b\|$$

$$\|u - \hat{u}\| \leq \|A^{-1}\| \cdot \|b - \hat{b}\|$$

$$\frac{\|u - \hat{u}\|}{\|u\|} \leq \frac{\|A^{-1}\| \cdot \|b - \hat{b}\|}{\|u\|}$$

Since $\|b\| = \|Au\| \leq \|A\| \cdot \|u\|$, $\|u\| \geq \frac{\|b\|}{\|A\|}$

$$\frac{\|u - \hat{u}\|}{\|u\|} \leq \frac{\|A\| \cdot \|A^{-1}\| \cdot \|b - \hat{b}\|}{\|b\|}$$

$$\boxed{\frac{\|u - \hat{u}\|}{\|u\|} \leq \kappa(A) \cdot \frac{\|b - \hat{b}\|}{\|b\|}}$$

(b)

$$A^{-1}r = A^{-1}Ae$$

$$e = A^{-1}r$$

$$\|e\| = \|A^{-1}r\| \leq \|A^{-1}\| \cdot \|r\|$$

$$\frac{\|e\|}{\|u\|} \leq \frac{\|A^{-1}\| \cdot \|r\|}{\|u\|}$$

Since $\|b\| = \|Au\| \leq \|A\| \cdot \|u\|$ so $\frac{1}{\|u\|} \leq \frac{\|A\|}{\|b\|}$:

$$\frac{\|e\|}{\|u\|} \leq \|A^{-1}\| \cdot \|r\| \cdot \frac{\|A\|}{\|b\|}$$

$$\frac{\|e\|}{\|u\|} \leq \|A\| \|A^{-1}\| \cdot \frac{\|r\|}{\|b\|}$$

$$\frac{\|e\|}{\|u\|} \leq \kappa(A) \cdot \frac{\|r\|}{\|b\|}$$

From $r = Ae$:

$$\|r\| = \|Ae\| \leq \|A\| \cdot \|e\|$$

$$\|e\| \geq \frac{\|r\|}{\|A\|}$$

$$\frac{\|e\|}{\|u\|} \geq \frac{\|r\|}{\|A\|} \cdot \frac{1}{\|u\|}$$

Since $u = A^{-1}b$, $\|u\| = \|A^{-1}b\| \leq \|A^{-1}\| \cdot \|b\|$ so $\frac{1}{\|u\|} \geq \frac{1}{\|A^{-1}\| \cdot \|b\|}$:

$$\frac{\|e\|}{\|u\|} \geq \frac{\|r\|}{\|A\|} \cdot \frac{1}{\|A^{-1}\| \cdot \|b\|}$$

$$\frac{\|e\|}{\|u\|} \geq \frac{1}{\|A\| \|A^{-1}\|} \cdot \frac{\|r\|}{\|b\|}$$

$$\frac{\|e\|}{\|u\|} \geq \frac{1}{\kappa(A)} \cdot \frac{\|r\|}{\|b\|}$$

Thus,

$$\boxed{\frac{1}{\kappa(A)} \frac{\|r\|}{\|b\|} \leq \frac{\|e\|}{\|u\|} \leq \kappa(A) \frac{\|r\|}{\|b\|}}$$

Interpretation: a smaller $\kappa(A)$ (i.e. well conditioned matrix) means the relationship between error e and residual r is tight. For a higher $\kappa(A)$, the relationship is less specific and a small r can mean a large e .

Problem 2

(a)

Let

$$(v_j)_i = \sin(j\pi x_i) = \sin\left(\frac{j\pi i}{m}\right), \quad i = 1, \dots, m-1.$$

$$(Av_j)_i = \frac{1}{h^2}(-(v_j)_{i-1} + 2(v_j)_i - (v_j)_{i+1})$$

$$(Av_j)_i = \frac{1}{h^2} \left(-\sin\left(\frac{j\pi(i-1)}{m}\right) + 2\sin\left(\frac{j\pi i}{m}\right) - \sin\left(\frac{j\pi(i+1)}{m}\right) \right).$$

Since $\sin(\alpha + \theta) + \sin(\alpha - \theta) = 2\sin(\alpha)\cos(\theta)$, with $\alpha = \frac{j\pi i}{m}$ and $\theta = \frac{j\pi}{m}$:

$$\begin{aligned} \sin\left(\frac{j\pi(i+1)}{m}\right) + \sin\left(\frac{j\pi(i-1)}{m}\right) &= 2\sin\left(\frac{j\pi i}{m}\right)\cos\left(\frac{j\pi}{m}\right). \\ (Av_j)_i &= \frac{1}{h^2} \left(2 - 2\cos\left(\frac{j\pi}{m}\right) \right) \sin\left(\frac{j\pi i}{m}\right). \end{aligned}$$

Thus

$$Av_j = \lambda_j v_j,$$

so vectors $\boxed{(v_j)_i = \sin(j\pi x_i)}$ are eigenvectors of A .

(b)

From (a) we know that $\lambda_j = \frac{1}{h^2} \left(2 - 2\cos\left(\frac{j\pi}{m}\right) \right)$.

Using $2 - 2\cos\theta = 4\sin^2(\theta/2)$,

$$\boxed{\lambda_j = \frac{4}{h^2} \sin^2\left(\frac{j\pi}{2m}\right), \quad j = 1, \dots, m-1.}$$

(c)

Since A is symmetric positive definite,

$$\kappa(A) = \frac{\lambda_{\max}}{\lambda_{\min}}.$$

$$\lambda_{\min} = \lambda_1 = \frac{4}{h^2} \sin^2\left(\frac{\pi}{2m}\right).$$

$$\lambda_{\max} = \lambda_{m-1} = \frac{4}{h^2} \sin^2\left(\frac{(m-1)\pi}{2m}\right) = \frac{4}{h^2} \cos^2\left(\frac{\pi}{2m}\right).$$

So:

$$\kappa(A) = \frac{\cos^2\left(\frac{\pi}{2m}\right)}{\sin^2\left(\frac{\pi}{2m}\right)} = \cot^2\left(\frac{\pi}{2m}\right).$$

As $m \rightarrow \infty$, $\frac{\pi}{2m} \rightarrow 0$ and $\sin \frac{\pi}{2m} \sim \frac{\pi}{2m} \sim 0$, $\cos \frac{\pi}{2m} \sim 1$:

$$\kappa(A) = \cot^2\left(\frac{\pi}{2m}\right) \sim \left(\frac{1}{\frac{\pi}{2m}}\right)^2 = \left(\frac{2m}{\pi}\right)^2.$$

Thus,

$$\boxed{\kappa(A) = O(m^2) \quad \text{as } m \rightarrow \infty.}$$

Problem 3

$$u(x) = \sin(k\pi x) + c\left(x - \frac{1}{2}\right)^3$$

$$u'(x) = k\pi \cdot \cos(k\pi x) + 3c\left(x - \frac{1}{2}\right)^2$$

$$u''(x) = -k^2\pi^2 \cdot \sin(k\pi x) + 6c\left(x - \frac{1}{2}\right)$$

$$-u''(x) + \gamma u(x) = f(x)$$

$$f(x) = -\left(-k^2\pi^2 \sin(k\pi x) + 6c\left(x - \frac{1}{2}\right)\right) + \gamma \left(\sin(k\pi x) + c\left(x - \frac{1}{2}\right)^3\right)$$

$$f(x) = k^2\pi^2 \sin(k\pi x) - 6c\left(x - \frac{1}{2}\right) + \gamma \sin(k\pi x) + \gamma c\left(x - \frac{1}{2}\right)^3$$

$$f(x) = (k^2\pi^2 + \gamma) \sin(k\pi x) - 6c\left(x - \frac{1}{2}\right) + \gamma c\left(x - \frac{1}{2}\right)^3$$

$$\boxed{f(x) = (k^2\pi^2 + \gamma) \sin(k\pi x) - 6c\left(x - \frac{1}{2}\right) + \gamma c\left(x - \frac{1}{2}\right)^3}$$

Problem 4

Note: in the results below, iteration 0 is not counted.

(a) 1000+. Did not meet required tolerances after 1000 iterations.

(b) 102 iterations.

(c) 1 iteration. This makes sense because without the cubic factor, the residual is enough for CG to descent in one iteration, because the RHS lies entirely in the span of one eigenvector of A.

(d) 1 iteration.

(e) 1 iteration.

(f) 1 iteration for both 1 and 2 processors.